$\displaystyle \lim_{n \to \infty} (\sqrt{4n^2 + 10n +2} -2n+5) =$

$\displaystyle \lim_{n \to \infty}\frac{(4n^2+10n+2)-(4n^2-20n+25)}{\sqrt{4n^2+10n+2}+2n-5} =$

$\displaystyle \lim_{n \to \infty} \frac{30n-23}{\sqrt{4n^2+10n+2}+2n-5}=$ 

$\displaystyle \lim_{n \to \infty} \frac{30-\frac{23}{n}}{\sqrt{4+\frac{10}{n}+\frac{2}{n^2}}+2-\frac{5}{n}}=\frac{30}{2+2}=\frac{15}{2}$



$$\begin{array}
\displaystyle \lim_{n \to \infty} (\sqrt{4n^2 + 10n +2} -2n+5) =\\\\
\lim_{n \to \infty}\frac{(4n^2+10n+2)-(4n^2-20n+25)}{\sqrt{4n^2+10n+2}+2n-5} = \\\\
lim_{n \to \infty} \frac{30n-23}{\sqrt{4n^2+10n+2}+2n-5}=\\\\
\lim_{n \to \infty} \frac{30-\frac{23}{n}}{\sqrt{4+\frac{10}{n}+\frac{2}{n^2}}+2-\frac{5}{n}}=\\=\frac{30}{2+2}=\frac{15}{2}
\end{array}
$$
